type/merge.v
@@ -5,28 +5,25 @@ From Paco Require Import paco pacotac.
 Require Import Setoid Morphisms Coq.Program.Basics.
 Require Import Coq.Init.Datatypes.
 
-Inductive merge2 : ltt -> ltt -> ltt -> Prop := 
-  | mrg_id : forall x, merge2 x x x
-  | mrg_bra : forall p xs ys IJ, 
-                Forall3S (fun u v w => 
-                  (u = None /\ v = None /\ w = None) \/
-                  (exists t, u = None /\ v = Some t /\ w = Some t) \/
-                  (exists t, u = Some t /\ v = None /\ w = Some t) \/
-                  (exists t, u = Some t /\ v = Some t /\ w = Some t)) xs ys IJ -> 
-                  SList xs -> SList ys ->
-              merge2 (ltt_recv p xs) (ltt_recv p ys) (ltt_recv p IJ).
 
 Inductive isMerge : ltt -> list (option ltt) -> Prop :=
   | matm : forall t, isMerge t (Some t :: nil)
   | mconsn : forall t xs, isMerge t xs -> isMerge t (None :: xs) 
-  | mconss : forall t t' t'' xs, isMerge t xs -> merge2 t t' t'' -> isMerge t'' (Some t' :: xs). 
+  | mconss : forall t xs, isMerge t xs -> isMerge t (Some t :: xs). 
 
 
 Lemma merge_end_back : forall ys0 t,
     Forall (fun u : option ltt => u = None \/ u = Some ltt_end) ys0 -> 
     isMerge t ys0 -> 
     t = ltt_end.
-Admitted.
+Proof.
+  induction ys0; intros; try easy.
+  inversion H. subst. inversion H0. subst. 
+  - destruct H3; try easy. inversion H1. subst. easy.
+  - subst. specialize(IHys0 t H4 H5). easy.
+  - subst. destruct H3; try easy. inversion H1. easy.
+Qed.
+
 
 Lemma Iso_mon : monotone2 lttIso.
 Proof.
@@ -93,31 +90,33 @@ Proof.
   intros t t' r ys0. revert t t' r.
   induction ys0; intros; try easy. destruct ys1; try easy.
   inversion H. subst. clear H.
-  inversion H0. subst. destruct ys1; try easy.
-  destruct H5; try easy. destruct H as (t1,(t2,(Ha,(Hb,Hc)))). inversion Ha. subst.
-  inversion H1. subst. easy. subst. inversion H4; try easy.
-  subst. destruct H5. destruct H. subst. inversion H1. subst.
-  specialize(IHys0 t t' r ys1 H7 H3 H5). easy.
-  destruct H as (t1,(t2,(Ha,(Hb,Hc)))). easy.
-  subst.
-  destruct H5; try easy. destruct H as (t1,(t2,(Ha,(Hb,Hc)))). inversion Ha. subst.
-  inversion H1. subst. inversion H0. subst. inversion H4. 
-  subst. destruct ys0; try easy. subst.
-  specialize(IHys0 t0 t3 r ys1 H7 H4 H5). clear H0 H1 H4 H5 H7 Ha.
-  
-  inversion H6. subst. inversion H8; try easy. subst. easy.
-  subst. pinversion IHys0; try easy. subst. 
-  apply lttIso_inv_b; try easy.
-  specialize(lttIso_inv Hc); intros. destruct H2. 
-  
-Admitted.
+  specialize(IHys0 t t' r ys1 H7).
+  inversion H0. subst. inversion H1. subst.
+  - destruct H5; try easy. destruct H as (t1,(t2,(Ha,(Hb,Hc)))). inversion Ha. inversion Hb. subst. easy.
+  - subst. destruct H5; try easy.
+    destruct H as (t1,(t2,(Ha,(Hb,Hc)))). easy.
+  - subst. destruct H5; try easy. destruct H as (t1,(t2,(Ha,(Hb,Hc)))). inversion Ha. inversion Hb. subst. easy.
+  - subst. inversion H1; try easy. subst. destruct H5; try easy.
+    destruct H as (t1,(t2,(Ha,(Hb,Hc)))). easy.
+  - subst. apply IHys0; try easy.
+  - subst. destruct H5; try easy. destruct H as (t1,(t2,(Ha,(Hb,Hc)))). easy.
+  - subst. destruct H5; try easy. destruct H as (t1,(t2,(Ha,(Hb,Hc)))). inversion Ha. subst. 
+    inversion H1. subst. easy. subst. easy.
+Qed.
 
 Lemma _a_29_part_helper_recv : forall n ys1 x4 p ys,
     onth n ys1 = Some x4 ->
     isMerge (ltt_recv p ys) ys1 -> 
     exists ys1', x4 = ltt_recv p ys1'.
-Proof. intro n.
-Admitted.
+Proof. 
+  induction n; intros; try easy.
+  - destruct ys1; try easy. simpl in *. subst. 
+    inversion H0. subst. exists ys. easy.
+    subst. exists ys. easy.
+  - destruct ys1; try easy.
+    specialize(IHn ys1 x4 p ys). apply IHn; try easy.
+    inversion H0; try easy. subst. destruct n; try easy.
+Qed.
 
 Lemma _a_29_part_helper_send : forall n ys2 x3 q x,
     onth n ys2 = Some x3 ->
@@ -128,8 +127,15 @@ Proof. intro n.
        - inversion H0. subst. simpl in H. inversion H. subst.
          exists x. easy.
          subst. simpl in H. easy.
-         subst. simpl in H. inversion H. subst. 
-Admitted.
+         subst. simpl in H. inversion H. subst.
+       - exists x. easy.
+       - destruct ys2; try easy.
+         inversion H0. subst. destruct n; try easy.
+         subst.
+         specialize(IHn ys2 x3 q x). apply IHn; try easy.
+         subst.
+         specialize(IHn ys2 x3 q x). apply IHn; try easy.
+Qed.
 
 Lemma triv_merge : forall T T', isMerge T (Some T' :: nil) -> T = T'.
 Proof. intros.
@@ -148,7 +154,11 @@ Qed.
 Lemma triv_merge3 : forall T xs, isMerge T xs -> isMerge T (Some T :: xs).
 Proof. intros.
        apply mconss with (t := T); try easy.
-       constructor. 
+Qed.
+
+Lemma merge_inv : forall T a xs, isMerge T (a :: xs) -> a = None \/ a = Some T.
+Proof.
+  intros. inversion H; subst; try easy. right. easy. left. easy. right. easy.
 Qed.
 
 (* needed *)
@@ -173,8 +183,8 @@ Proof.
   inversion H.
   - subst. constructor; try easy. right. easy.
   - subst. specialize(IHys0 H2). constructor; try easy. left. easy.
-  - subst. inversion H4. subst.
-    specialize(IHys0 H3). constructor; try easy. right. easy.
+  - subst. constructor; try easy. right. easy. 
+    apply IHys0; try easy.
 Qed.
 
 (* need *)
@@ -184,7 +194,15 @@ Lemma merge_label_recv : forall Mp LQ' LQ0' T k l p,
           onth l LQ0' = Some T ->
           exists T', onth l LQ' = Some T'.
 Proof. intros Mp.
-Admitted.
+  induction Mp; intros; try easy.
+  - inversion H. subst. 
+    destruct k; try easy. simpl in H0. inversion H0. subst. exists T. easy.
+  - simpl in H0. destruct k; try easy.
+  - subst. destruct k; try easy.
+    specialize(IHMp LQ' LQ0' T k l p). apply IHMp; try easy.
+  - subst. destruct k; try easy. simpl in H0. inversion H0. subst. exists T. easy.
+  - specialize(IHMp LQ' LQ0' T k l p). apply IHMp; try easy.
+Qed.
 
 (* need *)
 Lemma merge_label_send : forall Mq LP' LP0' T k l q,
@@ -193,7 +211,15 @@ Lemma merge_label_send : forall Mq LP' LP0' T k l q,
           onth l LP0' = Some T ->
           exists T', onth l LP' = Some T'. 
 Proof. intro Mq.
-Admitted.
+  induction Mq; intros; try easy.
+  - inversion H. subst. 
+    destruct k; try easy. simpl in H0. inversion H0. subst. exists T. easy.
+  - simpl in H0. destruct k; try easy.
+  - subst. destruct k; try easy.
+    specialize(IHMq LP' LP0' T k l q). apply IHMq; try easy.
+  - subst. destruct k; try easy. simpl in H0. inversion H0. subst. exists T. easy.
+  - specialize(IHMq LP' LP0' T k l q). apply IHMq; try easy.
+Qed.
 
 Lemma merge_label_sendb : forall ys0 LP LP' ST n l q,
       isMerge (ltt_send q LP) ys0 ->
@@ -201,22 +227,43 @@ Lemma merge_label_sendb : forall ys0 LP LP' ST n l q,
       onth l LP = Some ST ->
       onth l LP' = Some ST.
 Proof. intro ys0.
-Admitted.
+  induction ys0; intros; try easy.
+  - destruct n; try easy. 
+    - simpl in *. subst. 
+      inversion H. subst.
+      - easy.
+      - subst. easy.
+    - inversion H. subst.
+      destruct n; try easy.
+      subst. specialize(IHys0 LP LP' ST n l q). apply IHys0; try easy.
+      subst. specialize(IHys0 LP LP' ST n l q). apply IHys0; try easy.
+Qed.
 
 Lemma merge_constr : forall p LQ ys1 n,
           isMerge (ltt_recv p LQ) ys1 ->
           onth n ys1 = Some ltt_end ->
           False.
 Proof. intros p LQ ys1 n.
-Admitted.
+  revert ys1. induction n; intros; try easy.
+  - destruct ys1; try easy. simpl in H0. subst. inversion H; try easy.
+  - destruct ys1; try easy. 
+    inversion H. subst. destruct n; try easy.
+    - subst. specialize(IHn ys1). apply IHn; try easy.
+    - subst. specialize(IHn ys1). apply IHn; try easy.
+Qed.
 
 Lemma merge_consts : forall q LP ys0 n,
           isMerge (ltt_send q LP) ys0 -> 
           onth n ys0 = Some ltt_end -> 
           False.
 Proof. intros q LP ys0 n.
-Admitted.
-
+  revert ys0. induction n; intros; try easy.
+  - destruct ys0; try easy. simpl in H0. subst. inversion H; try easy.
+  - destruct ys0; try easy. 
+    inversion H. subst. destruct n; try easy.
+    - subst. specialize(IHn ys0). apply IHn; try easy.
+    - subst. specialize(IHn ys0). apply IHn; try easy.
+Qed.
 
 Lemma merge_slist : forall T ys, isMerge T ys -> SList ys.
 Proof. intros.
@@ -227,20 +274,33 @@ Proof. intros.
        easy. easy.
 Qed.
 
-
 Lemma merge_label_recv_s : forall Mp LQ' LQ0' T k l p,
           isMerge (ltt_recv p LQ') Mp ->
           onth k Mp = Some (ltt_recv p LQ0') ->
           onth l LQ0' = Some T ->
           onth l LQ' = Some T.
-Admitted.
+Proof.
+  induction Mp; intros; try easy.
+  - destruct k; try easy. simpl in H0. subst.
+    - inversion H. subst. easy. subst. easy.
+    - inversion H. subst. destruct k; try easy.
+      subst. specialize(IHMp LQ' LQ0' T k l p). apply IHMp; try easy.
+      subst. specialize(IHMp LQ' LQ0' T k l p). apply IHMp; try easy.
+Qed.
 
 Lemma merge_label_send_s : forall Mq LP' LP0' T k l q,
           isMerge (ltt_send q LP') Mq ->
           onth k Mq = Some (ltt_send q LP0') ->
           onth l LP0' = Some T ->
           onth l LP' = Some T. 
-Admitted.
+Proof.
+  induction Mq; intros; try easy.
+  - destruct k; try easy. simpl in H0. subst.
+    - inversion H. subst. easy. subst. easy.
+    - inversion H. subst. destruct k; try easy.
+      subst. specialize(IHMq LP' LP0' T k l q). apply IHMq; try easy.
+      subst. specialize(IHMq LP' LP0' T k l q). apply IHMq; try easy.
+Qed.
 
 Lemma merge_sorts : forall ys0 ys1 p q PT QT,
     Forall2
@@ -258,10 +318,24 @@ Lemma merge_sorts : forall ys0 ys1 p q PT QT,
     Forall2
       (fun u v : option (sort * ltt) =>
        u = None /\ v = None \/ (exists (s : sort) (g g' : ltt), u = Some (s, g) /\ v = Some (s, g'))) PT QT.
-Admitted.
- 
- 
- 
+Proof.
+  induction ys0; intros; try easy.
+  destruct ys1; try easy. inversion H. subst. clear H.
+  specialize(merge_inv (ltt_recv p QT) a ys0 H0); intros.
+  specialize(merge_inv (ltt_send q PT) o ys1 H1); intros.
+  
+  destruct H.
+  - subst. inversion H0. subst. 
+    destruct H2. subst. inversion H1. subst.
+    specialize(IHys0 ys1 p q PT QT). apply IHys0; try easy.
+    subst. destruct H5; try easy. destruct H as (l1,(l2,(Ha,Hb))). easy.
+  - subst.
+    destruct H2. subst. destruct H5; try easy.
+    destruct H as (l1,(l2,(Ha,Hb))). easy.
+    subst. destruct H5; try easy.
+    destruct H as (l1,(l2,(Ha,(Hb,Hc)))). inversion Ha. subst. inversion Hb. subst.
+    easy.
+Qed.
  
  
  
